a) $$ \sqrt{5} + \sqrt{5} = 2\sqrt{5} $$

b) $$ \frac{\sqrt{51}}{\sqrt{51}} = 1 $$

c) $$ 2\sqrt{25} + 3\sqrt{25} = 5\sqrt{25} = 25 $$

d) $$ -4\sqrt{7} + -4\sqrt{7} = -8\sqrt{7} $$

e) $$ -2\frac{\sqrt{193}}{\frac{\sqrt{193}}{\frac{\sqrt[3]{193}}{-3}}} = -6 $$

f) $$ 6+9+8+9+\frac{-3}{16}=31+\frac{-3}{16} $$

g) $$ (\frac{-4}{7})^2 + (\frac{-4}{7})^2 + (\frac{-4}{7})^2 + (\frac{-4}{7})^2 = 
    (\frac{-16}{49})+(\frac{-16}{49})+(\frac{-16}{49})+(\frac{-16}{49})
    =(64/196)=1/3
    $$

h) $$ (14-6)^2+(14-6)^2+(14-6)^2+(14-6)^2=8^2+8^2+8^2+8^2=256
    $$





uitleg : √16 - √9 + √4 = 4 - 3 + 2 = 3

Oefening
1. √4 + √1 =
2. √9 - √4 = 
3. √1 x √1 = 
4. √4 / √2 = 
5. √9 + √4 - √1 =
6. √16 x √1 / √4 =
7. √1 + √4 * √9 =
8. √16 - √9 + √4 =
9. √25 x √1 - √16 =
10. √36 / √6 + √9 =
11. √49 - √36 * √1 =
12. √64 + √9 - √16 =
13. √81 x √1 / √9 =
14. √100 - √81 + √16 =
15. √121 / √11 * √4 =
16. √144 + √16 - √64 =
17. √169 x √1 / √13 =
18. √196 - √121 + √36 =
19. √225 x √1 - √144 =
20. √256 / √16 + √49 =
